<?xml version="1.0" encoding="UTF-8"?>
<rdf:RDF xmlns="http://www.semanticweb.org/jdziu_000/ontologies/2017/5/elections/humanFactors#"
     xml:base="http://www.semanticweb.org/jdziu_000/ontologies/2017/5/elections/humanFactors"
     xmlns:fibo-fnd-rel-rel="http://www.omg.org/spec/EDMC-FIBO/FND/Relations/Relations/"
     xmlns:rdf="http://www.w3.org/1999/02/22-rdf-syntax-ns#"
     xmlns:owl="http://www.w3.org/2002/07/owl#"
     xmlns:xml="http://www.w3.org/XML/1998/namespace"
     xmlns:xsd="http://www.w3.org/2001/XMLSchema#"
     xmlns:skos="http://www.w3.org/2004/02/skos/core#"
     xmlns:rdfs="http://www.w3.org/2000/01/rdf-schema#"
     xmlns:fibo-fnd-aap-agt="http://www.omg.org/spec/EDMC-FIBO/FND/AgentsAndPeople/Agents/"
     xmlns:elections="http://www.semanticweb.org/jdziu_000/ontologies/2017/5/elections#">
    <owl:Ontology rdf:about="http://www.semanticweb.org/jdziu_000/ontologies/2017/5/elections/humanFactors">
        <owl:imports rdf:resource="http://nomagic.com/ontology/upper"/>
        <owl:imports rdf:resource="http://example.com/ontology/VVSG"/>
        <owl:imports rdf:resource="http://www.semanticweb.org/jdziu_000/ontologies/2017/5/elections"/>
        <owl:imports rdf:resource="http://www.omg.org/spec/EDMC-FIBO/FND/AgentsAndPeople/Agents/"/>
        <owl:imports rdf:resource="http://www.omg.org/spec/EDMC-FIBO/FND/Relations/Relations/"/>
        <owl:imports rdf:resource="http://www.w3.org/2004/02/skos/core"/>
    </owl:Ontology>
    


    <!-- 
    ///////////////////////////////////////////////////////////////////////////////////////
    //
    // Object Properties
    //
    ///////////////////////////////////////////////////////////////////////////////////////
     -->


    


    <!-- http://www.semanticweb.org/jdziu_000/ontologies/2017/5/elections/humanFactors#partOfBallotFormat -->


    <owl:ObjectProperty rdf:about="http://www.semanticweb.org/jdziu_000/ontologies/2017/5/elections/humanFactors#partOfBallotFormat">
        <rdfs:domain rdf:resource="http://www.semanticweb.org/jdziu_000/ontologies/2017/5/elections/humanFactors#DisplayFormat"/>
        <rdfs:range rdf:resource="http://www.semanticweb.org/jdziu_000/ontologies/2017/5/elections#BallotFormat"/>
        <rdfs:label rdf:datatype="http://www.w3.org/2001/XMLSchema#string">part of ballot format</rdfs:label>
    </owl:ObjectProperty>
    


    <!-- 
    ///////////////////////////////////////////////////////////////////////////////////////
    //
    // Classes
    //
    ///////////////////////////////////////////////////////////////////////////////////////
     -->


    


    <!-- http://www.semanticweb.org/jdziu_000/ontologies/2017/5/elections/humanFactors#AlternativeFormat -->


    <owl:Class rdf:about="http://www.semanticweb.org/jdziu_000/ontologies/2017/5/elections/humanFactors#AlternativeFormat">
        <rdfs:label rdf:datatype="http://www.w3.org/2001/XMLSchema#string">Alternative Format</rdfs:label>
        <skos:definition xml:lang="en">The ballot or accompanying information is said to be in an alternative format if it is in a representation other than the standard ballot language and format. Examples include, but are not limited to languages other than English, Braille, ASCII text, large print, recorded audio. (VVSG 1.1)</skos:definition>
    </owl:Class>
    


    <!-- http://www.semanticweb.org/jdziu_000/ontologies/2017/5/elections/humanFactors#AudioFormat -->


    <owl:Class rdf:about="http://www.semanticweb.org/jdziu_000/ontologies/2017/5/elections/humanFactors#AudioFormat">
        <rdfs:subClassOf rdf:resource="http://www.semanticweb.org/jdziu_000/ontologies/2017/5/elections/humanFactors#AlternativeFormat"/>
        <rdfs:subClassOf rdf:resource="http://www.semanticweb.org/jdziu_000/ontologies/2017/5/elections/humanFactors#DisplayFormat"/>
        <rdfs:label rdf:datatype="http://www.w3.org/2001/XMLSchema#string">Audio Format</rdfs:label>
    </owl:Class>
    


    <!-- http://www.semanticweb.org/jdziu_000/ontologies/2017/5/elections/humanFactors#DisplayFormat -->


    <owl:Class rdf:about="http://www.semanticweb.org/jdziu_000/ontologies/2017/5/elections/humanFactors#DisplayFormat">
        <rdfs:label rdf:datatype="http://www.w3.org/2001/XMLSchema#string">Display Format</rdfs:label>
        <skos:definition xml:lang="en">The way the voting system communicates ballot choices and other information. (Human Factors Group)</skos:definition>
    </owl:Class>
    


    <!-- http://www.semanticweb.org/jdziu_000/ontologies/2017/5/elections/humanFactors#EnhancedVisualFormat -->


    <owl:Class rdf:about="http://www.semanticweb.org/jdziu_000/ontologies/2017/5/elections/humanFactors#EnhancedVisualFormat">
        <rdfs:subClassOf rdf:resource="http://www.semanticweb.org/jdziu_000/ontologies/2017/5/elections/humanFactors#AlternativeFormat"/>
        <rdfs:subClassOf rdf:resource="http://www.semanticweb.org/jdziu_000/ontologies/2017/5/elections/humanFactors#VisualFormat"/>
        <rdfs:label rdf:datatype="http://www.w3.org/2001/XMLSchema#string">Enhanced Visual Format</rdfs:label>
        <skos:definition xml:lang="en">Visual display format options for displaying ballot choices and other information with the addition of personal choices such as text size and color contrast.</skos:definition>
    </owl:Class>
    


    <!-- http://www.semanticweb.org/jdziu_000/ontologies/2017/5/elections/humanFactors#VisualFormat -->


    <owl:Class rdf:about="http://www.semanticweb.org/jdziu_000/ontologies/2017/5/elections/humanFactors#VisualFormat">
        <rdfs:subClassOf rdf:resource="http://www.semanticweb.org/jdziu_000/ontologies/2017/5/elections/humanFactors#DisplayFormat"/>
        <rdfs:label rdf:datatype="http://www.w3.org/2001/XMLSchema#string">Visual Format</rdfs:label>
        <skos:definition xml:lang="en">A display format in which ballot choices and other information are displayed on screen or paper for perception using sight.</skos:definition>
    </owl:Class>
    


    <!-- 
    ///////////////////////////////////////////////////////////////////////////////////////
    //
    // Annotations
    //
    ///////////////////////////////////////////////////////////////////////////////////////
     -->


    <rdf:Description rdf:about="http://www.semanticweb.org/jdziu_000/ontologies/2017/5/elections/humanFactors">
        <rdfs:label rdf:datatype="http://www.w3.org/2001/XMLSchema#string">HumanFactors</rdfs:label>
    </rdf:Description>
</rdf:RDF>



<!-- Generated by the OWL API (version 5.0.2.20160507-1747) https://github.com/owlcs/owlapi/ -->





<!-- Warning: type declarations were not added automatically. -->


<!-- Generated using the No Magic Cameo Concept Modeler (18.0 SP12, build 2017 12 20 13:56 (3634)) on 2018-08-08 at 18:53:22 GMT -->